Update syntax of `semHalfBakery` and rename semantics to `ptrans`

semantics/semHalfBakeryScript.sml
@@ -4,7 +4,7 @@ open astHalfBakeryTheory
 
 val _ = new_theory "semHalfBakery";
 
-val _ = Datatype`
+Datatype:
   label = LTau proc varN
         | LCom proc varN proc varN
         | LComSend proc varN proc varN
@@ -13,9 +13,9 @@ val _ = Datatype`
         | LSelSend proc bool proc
         | LSelRecv proc bool proc
         | LLet varN proc (datum list -> datum) (varN list)
-`;
+End
 
-val freeprocs_def = Define`
+Definition freeprocs_def:
   freeprocs (LTau p n)             = {p}
 ∧ freeprocs (LCom p1 v1 p2 v2)     = {p1;p2}
 ∧ freeprocs (LSel p1 b p2)         = {p1;p2}
@@ -25,9 +25,9 @@ val freeprocs_def = Define`
 ∧ freeprocs (LSelSend p1 b p2)     = {p1;p2}
 ∧ freeprocs (LComRecv p v _)       = {p}
 ∧ freeprocs (LSelRecv p b _)       = {p}
-`;
+End
 
-val sender_def = Define`
+Definition sender_def:
   sender (LTau p n)             = NONE
 ∧ sender (LCom p1 v1 p2 v2)     = SOME p1
 ∧ sender (LSel p1 b p2)         = SOME p1
@@ -36,9 +36,9 @@ val sender_def = Define`
 ∧ sender (LSelSend p1 b p2)     = SOME p1
 ∧ sender (LComRecv p1 v1 _)     = NONE
 ∧ sender (LSelRecv p1 b1 _)     = NONE
-`;
+End
 
-val receiver_def = Define`
+Definition receiver_def:
   receiver (LTau p n)              = NONE
 ∧ receiver (LCom p1 v1 p2 v2)      = SOME p2
 ∧ receiver (LSel p1 b p2)          = SOME p2
@@ -47,9 +47,9 @@ val receiver_def = Define`
 ∧ receiver (LSelSend p1 b p2)      = SOME p2
 ∧ receiver (LComRecv p1 v1 _)      = SOME p1
 ∧ receiver (LSelRecv p1 b1 _)      = SOME p1
-`;
+End
 
-val written_def = Define`
+Definition written_def:
   written (LTau p n)             = NONE
 ∧ written (LCom p1 v1 p2 v2)     = SOME(v2,p2)
 ∧ written (LSel p1 b p2)         = NONE
@@ -58,9 +58,9 @@ val written_def = Define`
 ∧ written (LSelSend p1 b p2)     = NONE
 ∧ written (LComRecv p v _)       = SOME (v,p)
 ∧ written (LSelRecv p b _)       = NONE
-`;
+End
 
-val read_def = Define`
+Definition read_def:
   read (LTau p n)             = {(n,p)}
 ∧ read (LCom p1 v1 p2 v2)     = {(v1,p1)}
 ∧ read (LSel p1 b p2)         = {}
@@ -69,10 +69,10 @@ val read_def = Define`
 ∧ read (LSelSend p1 b p2)     = {}
 ∧ read (LComRecv p v _)       = {}
 ∧ read (LSelRecv p b _)       = {}
-`;
+End
 
 (* The set of all processes in a choreography *)
-val procsOf_def = Define`
+Definition procsOf_def:
   procsOf  Nil               = []
 ∧ procsOf (IfThen _ p l r)   = nub ([p] ++ procsOf l ++ procsOf r)
 ∧ procsOf (Com p _ q _ c)    = nub ([p;q] ++ procsOf c)
@@ -80,7 +80,7 @@ val procsOf_def = Define`
 ∧ procsOf (Sel p _ q c)      = nub ([p;q] ++ procsOf c)
 ∧ procsOf (PSel q (p,_) c)   = nub ([p;q] ++ procsOf c)
 ∧ procsOf (Let _ p _ _ c)    = nub ([p]   ++ procsOf c)
-`;
+End
 
 Theorem procsOf_all_distinct:
   ∀c. ALL_DISTINCT (procsOf c)
@@ -91,99 +91,99 @@ Proof
   \\ rw [procsOf_def,ALL_DISTINCT,all_distinct_nub]
 QED
 
-val (trans_rules,trans_ind,trans_cases) = Hol_reln `
+Inductive ptrans:
 
   (* Communication *)
   (∀s v1 p1 v2 p2 d c.
     FLOOKUP s (v1,p1) = SOME d
     ∧ p1 ≠ p2
-    ⇒ trans (s,Com p1 v1 p2 v2 c) (LCom p1 v1 p2 v2) (s |+ ((v2,p2),d),c))
+    ⇒ ptrans (s,Com p1 v1 p2 v2 c) (LCom p1 v1 p2 v2) (s |+ ((v2,p2),d),c))
 
   (* Partial communication *)
 ∧ (∀s v1 p1 v2 p2 d c.
     FLOOKUP s (v1,p1) = SOME d
     ∧ p1 ≠ p2
-    ⇒ trans (s,Com p1 v1 p2 v2 c) (LComSend p1 v1 p2 v2) (s,PCom p2 v2 (p1,d) c))
+    ⇒ ptrans (s,Com p1 v1 p2 v2 c) (LComSend p1 v1 p2 v2) (s,PCom p2 v2 (p1,d) c))
 
   (* Receive communication *)
 ∧ (∀s p1 v2 p2 d c.
     p1 ≠ p2
-    ⇒ trans (s,PCom p2 v2 (p1,d) c) (LComRecv p2 v2 (p1,d)) (s |+ ((v2,p2),d),c))
+    ⇒ ptrans (s,PCom p2 v2 (p1,d) c) (LComRecv p2 v2 (p1,d)) (s |+ ((v2,p2),d),c))
 
   (* Selection *)
 ∧ (∀s p1 b p2 c.
     p1 ≠ p2
-    ⇒ trans (s,Sel p1 b p2 c) (LSel p1 b p2) (s,c))
+    ⇒ ptrans (s,Sel p1 b p2 c) (LSel p1 b p2) (s,c))
 
   (* Partial selection *)
 ∧ (∀s p1 b p2 c.
     p1 ≠ p2
-    ⇒ trans (s,Sel p1 b p2 c) (LSelSend p1 b p2) (s,PSel p2 (p1,b) c))
+    ⇒ ptrans (s,Sel p1 b p2 c) (LSelSend p1 b p2) (s,PSel p2 (p1,b) c))
 
   (* Receive selection *)
 ∧ (∀s p1 b p2 c.
     p1 ≠ p2
-    ⇒ trans (s,PSel p2 (p1,b) c) (LSelRecv p2 b p1) (s,c))
+    ⇒ ptrans (s,PSel p2 (p1,b) c) (LSelRecv p2 b p1) (s,c))
 
   (* Let *)
 ∧ (∀s v p f vl c.
     EVERY IS_SOME (MAP (FLOOKUP s) (MAP (λv. (v,p)) vl))
-    ⇒ trans (s,Let v p f vl c)
+    ⇒ ptrans (s,Let v p f vl c)
             (LLet v p f vl)
             (s |+ ((v,p),f(MAP (THE o FLOOKUP s) (MAP (λv. (v,p)) vl))),c))
 
   (* If (True) *)
 ∧ (∀s v p c1 c2.
     FLOOKUP s (v,p) = SOME [1w]
-    ⇒ trans (s,IfThen v p c1 c2) (LTau p v) (s,c1))
+    ⇒ ptrans (s,IfThen v p c1 c2) (LTau p v) (s,c1))
 
   (* If (False) *)
 ∧ (∀s v p c1 c2.
     FLOOKUP s (v,p) = SOME w ∧ w ≠ [1w]
-    ⇒ trans (s,IfThen v p c1 c2) (LTau p v) (s,c2))
+    ⇒ ptrans (s,IfThen v p c1 c2) (LTau p v) (s,c2))
 
-  (* Swapping transitions / Structural congruence *)
+  (* Swapping ptransitions / Structural congruence *)
 ∧ (∀s v p c1 c2 s' c1' c2' alpha.
-    trans (s,c1) alpha (s',c1')
-    ∧ trans (s,c2) alpha (s',c2')
+    ptrans (s,c1) alpha (s',c1')
+    ∧ ptrans (s,c2) alpha (s',c2')
     ∧ p ∉ freeprocs alpha
-    ⇒ trans (s,IfThen v p c1 c2) alpha (s',IfThen v p c1' c2'))
+    ⇒ ptrans (s,IfThen v p c1 c2) alpha (s',IfThen v p c1' c2'))
 ∧ (∀s c s' c' p1 v1 p2 v2 alpha.
-    trans (s,c) alpha (s',c')
+    ptrans (s,c) alpha (s',c')
     ∧ p1 ∉ freeprocs alpha
     ∧ p2 ∉ freeprocs alpha
-    ⇒ trans (s,Com p1 v1 p2 v2 c) alpha (s',Com p1 v1 p2 v2 c'))
+    ⇒ ptrans (s,Com p1 v1 p2 v2 c) alpha (s',Com p1 v1 p2 v2 c'))
 ∧ (∀s c s' c' p1 b p2 alpha.
-    trans (s,c) alpha (s',c')
+    ptrans (s,c) alpha (s',c')
     ∧ p1 ∉ freeprocs alpha
     ∧ p2 ∉ freeprocs alpha
-    ⇒ trans (s,Sel p1 b p2 c) alpha (s',Sel p1 b p2 c'))
+    ⇒ ptrans (s,Sel p1 b p2 c) alpha (s',Sel p1 b p2 c'))
 ∧ (∀s c s' c' p v f vl alpha.
-    trans (s,c) alpha (s',c')
+    ptrans (s,c) alpha (s',c')
     ∧ p ∉ freeprocs alpha
-    ⇒ trans (s,Let v p f vl c) alpha (s',Let v p f vl c'))
-`;
+    ⇒ ptrans (s,Let v p f vl c) alpha (s',Let v p f vl c'))
+End
 
-val _ = zip [ "trans_com","trans_com_send","trans_com_recv"
-            , "trans_sel","trans_sel_send","trans_sel_recv"
-            , "trans_let","trans_if_true","trans_if_false"
-            , "trans_if_swap"
-            , "trans_com_swap"
-            , "trans_sel_swap"
-            , "trans_let_swap"
+val _ = zip [ "ptrans_com","ptrans_com_send","ptrans_com_recv"
+            , "ptrans_sel","ptrans_sel_send","ptrans_sel_recv"
+            , "ptrans_let","ptrans_if_true","ptrans_if_false"
+            , "ptrans_if_swap"
+            , "ptrans_com_swap"
+            , "ptrans_sel_swap"
+            , "ptrans_let_swap"
               ]
-            (CONJUNCTS trans_rules) |> map save_thm;
+            (CONJUNCTS ptrans_rules) |> map save_thm;
 
-val trans_pairind = save_thm("trans_pairind",
-  theorem"trans_strongind"
+val ptrans_pairind = save_thm("ptrans_pairind",
+  theorem"ptrans_strongind"
   |> Q.SPEC `λa0 a1 a2. P (FST a0) (SND a0) a1  (FST a2) (SND a2)`
   |> SIMP_RULE std_ss [FORALL_PROD]
   |> Q.GEN `P`
 );
 
 (* Reflexive transitive closure *)
-val trans_s_def = Define`
-  trans_s = RTC (λp q. ∃s. trans p s q)
-`;
+Definition ptrans_s_def:
+  ptrans_s = RTC (λp q. ∃s. ptrans p s q)
+End
 
 val _ = export_theory ()
